Hashtable fixes + proof for freeze_table.
If all threads have joined, freeze_table produces a hashtable in a state
consistent with the total history.

mailbox/hashtable1.c
@@ -92,12 +92,13 @@ void *f(void *arg){
   free(arg);
 
   for(int i = 0; i < 3; i++){
-    int r = add_item(i, 0);
+    int r = add_item(i + 1, 1);
     if(r) total++;
   }
 
   *res = total;
   release2(l);
+  return NULL;
 }
 
 int main(void){
@@ -110,6 +111,9 @@ int main(void){
     thread_locks[i] = l;
     results[i] = (int *) surely_malloc (sizeof(int));
     makelock((void *)l);
+  }
+
+  for(int i = 0; i < 3; i++){
     int *t = (int *) surely_malloc(sizeof(int));
     *t = i;
     spawn((void *)&f, (void *)t);
@@ -120,8 +124,10 @@ int main(void){
     acquire(l);
     freelock2(l);
     free(l);
-    int r = *(results[i]);
-    total += r;
+    int *r = results[i];
+    int i = *r;
+    free(r);
+    total += i;
   }
 
   int keys[ARRAY_SIZE], values[ARRAY_SIZE];
